src/lib/poly/Kuiper.Poly.Map.fst
@@ -1,0 +1,107 @@
+module Kuiper.Poly.Map
+
+(* Simple kernel: pointwise map of a function on an array. *)
+
+#lang-pulse
+
+open Kuiper
+module Vec = Pulse.Lib.Vec
+module SZ = Kuiper.SizeT
+module Array1 = Kuiper.Array1
+open Kuiper.Array1
+open Kuiper.Seq.Common
+
+open Kuiper.Tensor { ctlayout }
+open Kuiper.Tensor.Layout.Alg { l1_forward }
+
+ghost
+fn explode_setup
+  (#et : Type0)
+  (lena : nat)
+  (#l : Array1.layout lena)
+  (a : Array1.t et l)
+  (#s : erased (lseq et lena))
+  ()
+  norewrite
+  requires
+    (a |-> s)
+  ensures
+    (forall+ (bid : natlt lena).
+      Cell a bid |-> (Seq.index s bid)) **
+    pure (SZ.fits (layout_size l))
+{
+  Array1.pts_to_ref a;
+  Array1.explode a;
+}
+
+ghost
+fn explode_teardown
+  (#et : Type0)
+  (f : et -> et)
+  (lena : nat)
+  (#l : Array1.layout lena)
+  (a : Array1.t et l)
+  (#s : erased (lseq et lena))
+  ()
+  norewrite
+  requires
+    (forall+ (bid : natlt lena).
+      Cell a bid |-> (f (s @! bid))) **
+    pure (SZ.fits (layout_size l))
+  ensures
+    a |-> (seq_map f s <: lseq et lena)
+{
+  forevery_map
+    (fun (i:natlt lena) -> Cell a i |-> (f (s @! i)))
+    (fun (i:natlt lena) -> Cell a i |-> ((seq_map f s)@!i))
+    fn x { () };
+  Array1.implode a;
+}
+
+inline_for_extraction noextract
+fn kf_map
+  (#et : Type0)
+  (f : et -> et)
+  (#lena : erased nat)
+  (#l : Array1.layout lena) {| ctlayout l |}
+  (a : Array1.t et l)
+  (#s : erased (lseq et lena) )
+  (bid : szlt lena)
+  ()
+  requires
+    gpu **
+    Cell a (bid <: natlt lena) |-> (s@!bid) **
+    block_id lena bid
+  ensures
+    gpu **
+    Cell a (bid <: natlt lena) |-> (f (s@!bid)) **
+    block_id lena bid
+{
+  let x = Array1.read_cell a bid;
+  Array1.write_cell a bid (f x);
+}
+
+inline_for_extraction noextract
+let kmap
+  (#et : Type0)
+  (f: et -> et)
+  (lena : szp{ lena <= max_blocks })
+  (#l : Array1.layout lena) {| ctlayout l |}
+  (a : Array1.t et l)
+  (#_ : squash (Array1.is_global a))
+  (#s : erased (lseq et lena))
+  : kernel_desc
+      (requires a |-> s)
+      (ensures  a |-> lseq_map f s)
+= {
+    nblk = lena;
+    f = kf_map f a;
+
+    frame    = pure (SZ.fits (layout_size l));
+    teardown = explode_teardown f lena a;
+    setup    = explode_setup lena a;
+    kpre =  (fun (i:natlt lena) -> Cell a i |-> (s@!i));
+    kpost = (fun (i:natlt lena) -> Cell a i |-> (f (s@!i)));
+    kpost_sendable = solve;
+    kpre_sendable  = solve;
+  } <: kernel_desc_m_1 _ _
