src/lib/poly/Kuiper.Poly.Map.fsti
@@ -1,0 +1,26 @@
+module Kuiper.Poly.Map
+
+(* Simple kernel: pointwise map of a function on an array. *)
+
+#lang-pulse
+
+open Kuiper
+module Vec = Pulse.Lib.Vec
+module SZ = Kuiper.SizeT
+module Array1 = Kuiper.Array1
+open Kuiper.Array1
+open Kuiper.Seq.Common
+open Kuiper.Tensor
+
+inline_for_extraction noextract
+val kmap
+  (#et : Type0)
+  (f: et -> et)
+  (lena : szp{ lena <= max_blocks })
+  (#l : Array1.layout lena) {| ctlayout l |}
+  (a : Array1.t et l)
+  (#_ : squash (Array1.is_global a))
+  (#s : erased (lseq et lena))
+  : kernel_desc
+      (requires a |-> s)
+      (ensures  a |-> lseq_map f s)
